Have constructed steps in Oeuf, and translated them to Cminor steps

src/Linker.v
@@ -4,6 +4,8 @@ Require Import compcert.common.Globalenvs.
 Require Import compcert.backend.Cminor.
 Require Import compcert.common.Errors.
 Require Import compcert.common.Values.
+Require Import compcert.lib.Maps.
+Require Import compcert.common.Memory.
 
 Require Import StructTact.StructTactics.
 Require Import StructTact.Util.
@@ -66,17 +68,67 @@ Fixpoint link_fundefs (l l' : list (ident * globdef Cminor.fundef unit)) : res (
     end
   end.
     
-           
+
+
+
+Fixpoint only_malloc_ext (l : list (ident * globdef Cminor.fundef unit)) : bool :=
+  match l with
+  | nil => true
+  | (id,Gfun (Internal _)) :: l' => only_malloc_ext l'
+  | (id,Gfun (External ef)) :: l' => if external_function_eq ef EF_malloc then
+                                       only_malloc_ext l' else
+                                       false
+  | (id,Gvar _ ) :: l' => false
+  end.
+
+Fixpoint no_builtin (s : Cminor.stmt) : Prop :=
+  match s with
+  | Sbuiltin _ _ _ => False
+  | Sseq s1 s2 => no_builtin s1 /\ no_builtin s2
+  | Sifthenelse _ s1 s2 => no_builtin s1 /\ no_builtin s2
+  | Sloop s => no_builtin s
+  | Sblock s => no_builtin s
+  | Slabel _ s => no_builtin s
+  | _ => True
+  end.
+
+Lemma no_builtin_dec :
+  forall s,
+    { no_builtin s } + { ~ no_builtin s }.
+Proof.
+  induction s; intros; simpl; auto;
+  destruct IHs1; destruct IHs2; eauto; try firstorder.
+Defined.
+
+Definition no_builtin_fundef (x : (ident * globdef Cminor.fundef unit)) : Prop :=
+  match x with
+  | (id,Gfun (Internal f)) => no_builtin (fn_body f)
+  | _ => True
+  end.
+
+Lemma no_builtin_fundef_dec :
+  forall x,
+    { no_builtin_fundef x } + { ~ no_builtin_fundef x }.
+Proof.
+  intros. destruct x. destruct g; simpl; auto.
+  destruct f; simpl; auto.
+  eapply no_builtin_dec; eauto.
+Defined.
+
 (* We need a way to construct a shim, given Oeuf code *)
 Definition shim_link (oeuf_code : Cminor.program) (shim_code : Cminor.program) : res Cminor.program :=
   if (list_norepet_dec peq (prog_defs_names oeuf_code)) then
     if (list_norepet_dec peq (prog_defs_names shim_code)) then
+      if (only_malloc_ext (prog_defs oeuf_code)) then
+        if (Forall_dec no_builtin_fundef no_builtin_fundef_dec (prog_defs oeuf_code)) then
   match (link_fundefs (prog_defs oeuf_code) (prog_defs shim_code)) with
   | OK fds => OK (AST.mkprogram fds
                                     (prog_public shim_code)
                                     (prog_main shim_code))
   | Error m => Error m
   end
+    else Error ((MSG "Oeuf code somehow has builtins") :: nil)
+      else Error ((MSG "Oeuf code contained non-malloc external functions, or global variables") :: nil)
     else Error ((MSG "Shim list_norepet check failed"):: nil)
   else Error ((MSG "Oeuf list_norepet check failed"):: nil).
 
@@ -358,16 +410,35 @@ Section LINKED.
   Definition shim_ge := Genv.globalenv shim_code.
   Definition link_ge := Genv.globalenv link_code.
 
-  Lemma oeuf_ident_transf :
-    forall id fd b,
+  Lemma oeuf_symbol_transf :
+    forall id b,
       Genv.find_symbol oeuf_ge id = Some b ->
-      Genv.find_funct_ptr oeuf_ge b = Some fd ->
-      Genv.find_symbol link_ge id = Some b /\ Genv.find_funct_ptr link_ge b = Some fd.
+      Genv.find_symbol link_ge id = Some b.
   Proof.
-    intros.
-    (* This is true due to how the linker is defined *)
+  Admitted.
+
+  Lemma oeuf_funct_ptr_transf :
+    forall b fd,
+      Genv.find_funct_ptr oeuf_ge b = Some fd ->
+      Genv.find_funct_ptr link_ge b = Some fd.
+  Proof.
+  Admitted.
+
+  Definition internal_or_malloc (fd : fundef) : Prop :=
+    match fd with
+    | Internal _ => True
+    | External ef => ef = EF_malloc
+    end.
+
+  Lemma oeuf_funs_internal :
+    forall b fd,
+      Genv.find_funct_ptr oeuf_ge b = Some fd ->
+      internal_or_malloc fd.
+  Proof.
   Admitted.
       
+  
+
 (*  
   Lemma oeuf_ident_transf_weak :
     forall id fd,
@@ -400,37 +471,397 @@ Section LINKED.
   (* We'll use the fact that we linked up *)
   (* to show that we simply never made any external calls *)
 
-
-  (*
-    Lemma eval_expr_transf :
-      forall sp e m a v,
-        eval_expr oeuf_ge sp e m a v ->
-        exists v',
-          eval_expr link_ge sp e m a v' /\ Val.lessdef v v'.
-    Proof.
-      induction 1; intros;
-        try solve [eexists; split; try econstructor; eauto].
-      eexists; split; try econstructor; eauto.
-      
-
-  
-  Lemma step_sim :
-    forall st t st',
-      step oeuf_ge st t st' ->
-      step link_ge st t st'.
-  Proof.
-    intros.
-    inv H; try solve [econstructor; eauto].
-*)
-    
-
   (* TODO: shim should have i64 definitions *)
   (* no need to manually add them *)
   (* Use the fact that Oeuf before only had malloc to show that steps are well behaved *)
   (* and to create a simple simulation argument *)
   (* that doesn't need Mem.inject or anything (same memory) *)
+
   
   
+  Definition env_lessdef (e e' : env) : Prop :=
+    forall id v,
+      e ! id = Some v ->
+      exists v',
+        e' ! id = Some v' /\ Val.lessdef v v'.
+      
+
+  Inductive match_cont : cont -> cont -> Prop :=
+  | match_stop :
+      match_cont Kstop Kstop
+  | match_seq :
+      forall s k k',
+        match_cont k k' ->
+        no_builtin s ->
+        match_cont (Kseq s k) (Kseq s k')
+  | match_block :
+      forall k k',
+        match_cont k k' ->
+        match_cont (Kblock k) (Kblock k')
+  | match_call :
+      forall k k' oid f v v' e e',
+        match_cont k k' ->
+        Val.lessdef v v' ->
+        env_lessdef e e' ->
+        no_builtin (fn_body f) ->
+        match_cont (Kcall oid f v e k) (Kcall oid f v' e' k').
+                   
+
+  
+  Inductive match_states : state -> state -> Prop :=
+  | match_state :
+      forall f s k k' v v' e e' m m',
+        env_lessdef e e' ->
+        Mem.extends m m' ->
+        Val.lessdef v v' ->
+        match_cont k k' ->
+        no_builtin s ->
+        no_builtin (fn_body f) ->
+        match_states (State f s k v e m) (State f s k' v' e' m')
+  | match_callstate :
+      forall fd vs vs' k k' m m',
+        Val.lessdef_list vs vs' ->
+        match_cont k k' ->
+        Mem.extends m m' ->
+        internal_or_malloc fd ->
+        match fd with
+        | Internal f => no_builtin (fn_body f)
+        | _ => True
+        end ->
+        match_states (Callstate fd vs k m) (Callstate fd vs' k' m')
+  | match_returnstate :
+      forall v v' k k' m m',
+        Val.lessdef v v' ->
+        match_cont k k' ->
+        Mem.extends m m' ->
+        match_states (Returnstate v k m) (Returnstate v' k' m').
+
+  Lemma eval_unop_transf :
+    forall op x x' v,
+      eval_unop op x = Some v ->
+      Val.lessdef x x' ->
+      exists v',
+        eval_unop op x' = Some v' /\ Val.lessdef v v'.
+  Proof.
+    induction op; intros; simpl in H; try find_inversion;
+      try solve [eexists; split; simpl; try reflexivity;
+                 try eapply Val.zero_ext_lessdef;
+                 try eapply Val.sign_ext_lessdef;
+                 eauto].
+  Admitted.
+
+  Lemma eval_binop_transf :
+    forall op v1 v2 m v v1' v2' m',
+      eval_binop op v1 v2 m = Some v ->
+      Mem.extends m m' ->
+      Val.lessdef v1 v1' ->
+      Val.lessdef v2 v2' ->
+      exists v',
+        eval_binop op v1' v2' m' = Some v' /\ Val.lessdef v v'.
+  Proof.
+  Admitted.
+  
+  Lemma eval_expr_transf :
+    forall sp sp' e e' m m' a v,
+      eval_expr oeuf_ge sp e m a v ->
+      Val.lessdef sp sp' ->
+      env_lessdef e e' ->
+      Mem.extends m m' ->
+      exists v',
+        eval_expr link_ge sp' e' m' a v' /\ Val.lessdef v v'.
+  Proof.
+    induction 1; intros.
+
+    eapply H1 in H. break_exists; break_and.
+    exists x; split; try econstructor; eauto.
+
+    destruct cst; simpl in *; try find_inversion; try break_match;
+      try eapply oeuf_symbol_transf in Heqo;
+      try solve [eexists; split; econstructor; eauto].
+    eexists; split. econstructor; eauto. simpl. collapse_match. reflexivity.
+    econstructor; eauto.
+    destruct (Genv.find_symbol link_ge i) eqn:?.
+    eexists; split. econstructor; eauto. simpl. collapse_match. reflexivity.
+    econstructor; eauto.
+    eexists; split. econstructor; eauto. simpl. collapse_match. reflexivity.
+    econstructor; eauto.
+    eexists; split. econstructor; eauto. simpl. reflexivity.
+    eapply Val.add_lessdef; eauto.
+    destruct IHeval_expr; eauto. break_and.
+    eapply eval_unop_transf in H0. instantiate (1 := x) in H0.
+    break_exists; break_and.
+    exists x0.
+    split; try econstructor; eauto. eassumption.
+    destruct IHeval_expr1; eauto.
+    destruct IHeval_expr2; eauto.
+    repeat break_and.
+    eapply eval_binop_transf in H1; eauto.
+    break_exists; break_and.
+    exists x1. split; try econstructor; eauto.
+    destruct IHeval_expr; eauto.
+    break_and.
+    eapply Mem.loadv_extends in H0; eauto.
+    break_exists. break_and.
+    exists x0. split; try econstructor; eauto.
+  Qed.
+
+  Lemma eval_exprlist_transf :
+    forall sp sp' e e' m m' expl vl,
+      eval_exprlist oeuf_ge sp e m expl vl ->
+      Val.lessdef sp sp' ->
+      env_lessdef e e' ->
+      Mem.extends m m' ->
+      exists vl',
+        eval_exprlist link_ge sp' e' m' expl vl' /\ Val.lessdef_list vl vl'.
+  Proof.
+  Admitted.
+
+  
+  Lemma match_is_call_cont :
+    forall k k',
+      match_cont k k' ->
+      is_call_cont k ->
+      is_call_cont k'.
+  Proof.
+    induction 1; intros; simpl in *;
+      try invp False;
+      eauto.
+  Qed.
+
+  Lemma env_lessdef_set :
+    forall e e',
+      env_lessdef e e' ->
+      forall id v v',
+        Val.lessdef v v' ->
+        env_lessdef (PTree.set id v e) (PTree.set id v' e').
+  Proof.
+  Admitted.
+
+  Lemma find_funct_transf :
+    forall vf vf' fd,
+      Genv.find_funct oeuf_ge vf = Some fd ->
+      Val.lessdef vf vf' ->
+      Genv.find_funct link_ge vf' = Some fd.
+  Proof.
+    intros. unfold Genv.find_funct in *.
+    repeat break_match_hyp; try congruence.
+    subst. inv H0.
+    break_match; try congruence.
+    eapply oeuf_funct_ptr_transf; eauto.
+  Qed.
+
+  Lemma match_call_cont :
+    forall k k',
+      match_cont k k' ->
+      match_cont (call_cont k) (call_cont k').
+  Proof.
+    induction 1; intros; simpl; try econstructor; eauto.
+  Qed.
+
+  Lemma find_funct_internal :
+    forall vf fd,
+      Genv.find_funct oeuf_ge vf = Some fd ->
+      internal_or_malloc fd.
+  Proof.
+    intros.
+    unfold Genv.find_funct in *.
+    repeat break_match_hyp; try congruence.
+    eapply oeuf_funs_internal; eauto.
+  Qed.
+
+  Lemma find_label_match_cont :
+    forall l s k s' k',
+      find_label l s k = Some (s',k') ->
+      no_builtin s ->
+      forall k0,
+        match_cont k k0 ->
+        exists k'0,
+          find_label l s k0 = Some (s',k'0) /\ match_cont k' k'0 /\ no_builtin s'.
+  Proof.
+  Admitted.
+
+  Lemma oeuf_no_builtin :
+    forall b fd,
+      Genv.find_funct_ptr oeuf_ge b = Some fd ->
+      match fd with
+      | Internal f0 => no_builtin (fn_body f0)
+      | External _ => True
+      end.
+  Proof.
+  Admitted.
+  
+
+  Lemma env_lessdef_set_params :
+    forall l vs vs',
+      Val.lessdef_list vs vs' ->
+      env_lessdef (set_params vs l) (set_params vs' l).
+  Proof.
+  Admitted.
+  
+  Lemma env_lessdef_set_locals :
+    forall e e',
+      env_lessdef e e' ->
+      forall l,
+        env_lessdef (set_locals l e) (set_locals l e').
+  Proof.
+  Admitted.
+
+  
+  Lemma step_sim :
+    forall st t st' lst,
+      step oeuf_ge st t st' ->
+      match_states st lst ->
+      exists lst',
+        step link_ge lst t lst' /\ match_states st' lst'.
+  Proof.
+    intros.
+    inv H; inv H0; try solve [eexists; split; econstructor; eauto];
+      try solve [invp match_cont; eexists; split; econstructor; eauto].
+      
+    - invp Val.lessdef.
+      eapply Mem.free_parallel_extends in H2; eauto.
+      break_exists; break_and.
+      eexists; split. econstructor; eauto.
+      eapply match_is_call_cont; eauto.
+      econstructor; eauto.
+
+    - eapply eval_expr_transf in H1; eauto.
+      break_exists; break_and.
+      
+      eexists; split. econstructor; eauto.
+      econstructor; eauto.
+      eapply env_lessdef_set; eauto.
+
+    - eapply eval_expr_transf in H1; eauto.
+      eapply eval_expr_transf in H2; eauto.
+      repeat break_exists; repeat break_and.
+      eapply Mem.storev_extends in H3; eauto.
+      break_exists; break_and.
+      eexists; split. econstructor; eauto.
+      econstructor; eauto.
+
+    - eapply eval_expr_transf in H1; eauto.
+      eapply eval_exprlist_transf in H2; eauto.
+      
+      repeat break_exists; repeat break_and.
+      unfold Genv.find_funct in *.
+      repeat break_match_hyp; try congruence. subst.
+      inv H5.      
+      eexists; split. econstructor; eauto.
+      simpl. break_match; try congruence.
+      eapply oeuf_funct_ptr_transf; eauto.
+      econstructor; eauto. econstructor; eauto.
+      eapply oeuf_funs_internal; eauto.
+      eapply oeuf_no_builtin; eauto.
+      
+    - eapply eval_expr_transf in H1; eauto.
+      eapply eval_exprlist_transf in H2; eauto.
+      repeat break_exists; repeat break_and.
+      eapply Mem.free_parallel_extends in H5; eauto.
+      break_exists; break_and.
+      inv H14.
+      eexists; split. econstructor; eauto.
+      eapply find_funct_transf; eauto.
+      econstructor; eauto.
+      eapply match_call_cont; eauto.
+      eapply find_funct_internal; eauto.
+      unfold Genv.find_funct in *.
+      repeat (break_match_hyp; try congruence).
+      eapply oeuf_no_builtin; eauto.
+
+      
+    - simpl in *. invp False.
+
+    - simpl in *. break_and.
+      eexists; split. econstructor; eauto.
+      econstructor; eauto.
+      econstructor; eauto.
+
+    - simpl in *.
+      break_and.
+      eapply eval_expr_transf in H1; eauto.
+      break_exists; break_and.
+      inv H2; inv H5.
+      break_match;
+        eexists; split; repeat (econstructor; eauto).
+
+    - simpl in *.
+      eexists; split; repeat (econstructor; eauto).
+
+    - simpl in *.
+      eexists; split; repeat (econstructor; eauto).
+
+
+    - eapply eval_expr_transf in H1; eauto.
+      break_exists; break_and.
+      inv H2; inv H3.
+      eexists; split; repeat (econstructor; eauto).
+      eexists; split; repeat (econstructor; eauto).
+
+    - inv H11.
+      eapply Mem.free_parallel_extends in H1; eauto.
+      break_exists; break_and.
+      eexists; split; repeat (econstructor; eauto).
+      eapply match_call_cont; eauto.
+
+    - inv H12.
+      eapply eval_expr_transf in H1; eauto.
+      break_exists; break_and.
+      eapply Mem.free_parallel_extends in H2; eauto.
+      break_exists; break_and.
+      eexists; split; repeat (econstructor; eauto).
+      eapply match_call_cont; eauto.
+
+    - eapply find_label_match_cont in H1; eauto;
+        try eapply match_call_cont; eauto.
+      break_exists; break_and.
+      eexists; split; repeat (econstructor; eauto).
+
+    - eapply Mem.alloc_extends in H1; eauto.
+      break_exists. break_and.
+      Focus 2. instantiate (1 := 0). omega.
+      Focus 2. instantiate (1 := fn_stackspace f). omega.
+      eexists; split. econstructor; eauto.
+      econstructor; eauto.
+
+      eapply env_lessdef_set_locals; try eapply env_lessdef_set_params; eauto.
+
+    - simpl in H10. subst ef.
+      inv H1. invc H6. invc H8. invc H12.
+      eapply Mem.alloc_extends in H2; eauto.
+      Focus 2. instantiate (1 := -4); omega.
+      Focus 2. instantiate (1 := Integers.Int.unsigned n); omega.
+      break_exists. break_and.
+      eapply Mem.store_within_extends in H3; eauto.
+      break_exists. break_and.
+      eexists; split. econstructor; eauto.
+      econstructor; eauto.
+      econstructor; eauto.
+
+    - invp match_cont.
+      eexists; split.
+      econstructor; eauto.
+      econstructor; eauto; simpl; eauto.
+      destruct optid; simpl; eauto; eapply env_lessdef_set; eauto.
+      
+  Qed.
+    
+
+  Lemma star_step_sim :
+    forall st t st',
+      Smallstep.star step oeuf_ge st t st' ->
+      forall lst,
+        match_states st lst ->
+        exists lst',
+          Smallstep.star step link_ge lst t lst' /\ match_states st' lst'.
+  Proof.
+    induction 1; intros. eexists; split; try econstructor; eauto.
+    eapply step_sim in H; eauto. break_exists; break_and.
+    edestruct IHstar; eauto.
+    break_and. eexists; split. econstructor; eauto.
+    eauto.
+  Qed.
+    
 
 End LINKED.  
   
